ulib/ml/hyperheap/FStar_HyperHeap.ml
@@ -5,3 +5,4 @@ let root = ()
 type ('a, 'b, 'c) fresh_region = unit
 let extends a b = true
 let as_ref i r = r
+let sel _ = failwith "nope"
